Add hints to simple lemmas

Game/FormalLanguages/BasicDefinitions.lean
@@ -14,7 +14,6 @@ inductive Word where
 def w₁ := Word.cons 'a' (Word.cons 'b' .ε)
 def w₂ := Word.cons 'b' (Word.cons 'b' (Word.cons 'a' .ε))
 
-@[simp]
 def Word.chars : (w : Word) → Set Char
   | ε => ∅
   | cons s w => {s} ∪ w.chars
@@ -24,7 +23,6 @@ structure Language where
   Words : Set Word
   word_constraint : ∀ word ∈ Words, word.chars ⊆ Alphabet
 
-@[simp]
 def Word.count (w : Word) (s' : Char) : ℕ := match w with
   | .ε => 0
   | .cons s w => if (s = s') then 1 + w.count s' else w.count s'
@@ -33,72 +31,18 @@ def Word.count (w : Word) (s' : Char) : ℕ := match w with
 theorem count_uneq (w u : Word) : (∃ (s : Char), w.count s ≠ u.count s) → w ≠ u := by
   aesop
 
-@[simp]
 def Word.length : (w : Word) → ℕ
  | .ε => 0
  | .cons _ w => 1 + w.length
 
 macro:max (priority := 1001) atomic("|" noWs) a:term noWs "|" : term => `(Word.length $a)
 
-@[simp]
 def Word.cat (x y : Word) : Word :=
   match x with
  | .ε => y
  | .cons s x => .cons s (x.cat y)
 
 infixr:90 " ∘ " => Word.cat
---#reduce w₁ ∘ w₂
-
-@[simp]
-lemma Word.cat_eps (w : Word) : w ∘ .ε = w := by
-  induction' w with s w ih
-  · rw [cat]
-  · rw [cat, ih]
-
-@[simp]
-lemma Word.cat_assoc (x y z : Word) : (x ∘ y) ∘ z = x ∘ y ∘ z := by
-  induction' x with s w ih <;> simp_all only [cat]
-
-@[simp]
-lemma Word.cat_count {s : Char} (x y : Word) :
-    (x ∘ y).count s = x.count s + y.count s := by
-  induction' x with s' w ih
-  · simp_all only [cat, count, Nat.zero_add]
-  · rw [count]
-    simp_all only [cat, count]
-    split
-    next h =>
-      omega
-    next h => simp_all only
-
-@[simp]
-lemma Word.cat_count_zero {s : Char} (x y : Word) :
-    (x ∘ y).count s = 0 → x.count s = 0 ∧ y.count s = 0 := by
-  intro hcatcount
-  apply And.intro <;> simp_all only [cat_count, Nat.add_eq_zero_iff]
-
-@[simp]
-lemma Word.cat_chars (x y : Word) : (x ∘ y).chars = x.chars ∪ y.chars := by
-  induction' x with s w ih
-  · simp only [cat, chars, Set.empty_union]
-  · aesop
-
-lemma Word.cat_char_subset_left (x y : Word) :
-    x.chars ⊆ (x ∘ y).chars := by
-  simp only [cat_chars, Set.subset_union_left]
-
-lemma Word.cat_char_subset_right (x y : Word) :
-    y.chars ⊆ (x ∘ y).chars := by
-  simp only [cat_chars, Set.subset_union_right]
-
-lemma Word.cat_len (x y : Word) :
-    |(x ∘ y)| = |x| + |y| := by
-  induction' x with s x ih
-  · simp only [cat, length, Nat.zero_add]
-  · rw [Word.length, Nat.add_assoc, ← ih]
-    simp_all only [length]
-
-@[simp]
 def Word.pow (w : Word) (n : ℕ) : Word :=
   match n with
   | 0 => .ε
@@ -106,51 +50,31 @@ def Word.pow (w : Word) (n : ℕ) : Word :=
 
 infix:92 " ^ " => Word.pow
 
---#reduce w₁ ^ 3
-
-@[simp]
 def Symbol.pow (a : Char) (n : ℕ) : Word :=
   match n with
   | 0 => .ε
   | .succ n => .cons a (Symbol.pow a n)
 
-infix:91 " ^+^ " => Symbol.pow
+infix:93 " ^ " => Symbol.pow
+lemma Word.cat_chars (x y : Word) : (x ∘ y).chars = x.chars ∪ y.chars := by
+  induction' x with s w ih
+  · simp only [cat, chars, Set.empty_union]
+  · rw [chars, cat, chars, ih]
+    rw [Set.union_assoc]
 
-@[simp]
-lemma Symbol.pow_len {s : Char} (n : ℕ) : |s ^+^ n| = n := by
-  induction' n with n ih
-  · rfl
-  · simp only [pow, Word.length]
-    rw [ih]
-    exact Nat.one_add _
-
-@[simp]
-lemma Symbol.pow_chars {s : Char} {n : ℕ} (hn : n > 0) : (s ^+^ n).chars = {s} := by
+lemma Symbol.pow_chars {s : Char} {n : ℕ} (hn : n > 0) : (s ^ n).chars = {s} := by
   induction' n, hn using Nat.le_induction with n
   · simp_all only [Word.chars, Set.union_empty]
   · simp_all only [Word.chars, add_eq, Nat.add_zero, Set.union_self]
 
-@[simp]
-lemma Symbol.pow_count {s₁ s₂ : Char} (n : ℕ) :
-    (s₁ ^+^ n).count s₂ = if s₁ = s₂ then n else 0 := by
-  induction' n with n ih
-  · simp_all only [pow, Word.count, ite_self]
-  · simp_all only [pow, Word.count, ↓reduceIte]
-    split
-    next h =>
-      subst h
-      simp_all only [↓reduceIte]
-      omega
-    next h => simp_all only [↓reduceIte]
-
-def anbn : Set Word := {w | ∃ n, w = 'a' ^+^ n ∘ 'b' ^+^ n}
+def anbn : Set Word := {w | ∃ n : ℕ, w = ('a' ^ n) ∘ ('b' ^ n)}
 def anbn_lang : Language := ⟨{'a', 'b'}, anbn,
   by
     intro w hw c hc
     rw [anbn] at hw
     simp_all only [Set.mem_setOf_eq, Set.mem_insert_iff, Set.mem_singleton_iff, ↓Char.isValue]
     rcases hw with ⟨n, hw⟩
-    have hchars : w.chars = ('a' ^+^ n ∘ 'b' ^+^ n).chars := by rw [hw]
+    have hchars : w.chars = (('a' ^ n) ∘ 'b' ^ n).chars := by rw [hw]
     simp only [↓Char.isValue, Word.cat_chars] at hchars
     rw [hchars] at hc
     simp at hc
@@ -167,9 +91,9 @@ def anbn_lang : Language := ⟨{'a', 'b'}, anbn,
 
 set_option linter.unusedVariables false
 
-@[simp]
 def pumping_property (L : Language) :=
-  ∃ (n : ℕ) (hpos : n > 0),
+  ∃ (n : ℕ),
+  n > 0 ∧
   ∀ z ∈ L.Words,
   (hlen : z.length > n) →
     ∃ (u v w : Word),
@@ -177,126 +101,3 @@ def pumping_property (L : Language) :=
       |u ∘ v| ≤ n ∧
       |v| ≥ 1 ∧
       ∀ (i : ℕ), u ∘ v ^ i ∘ w ∈ L.Words
-
---set_option tactic.simp.trace true
-lemma Word.cons_a (n : ℕ) (x y z : Word) (hz : x ∘ y = 'a' ^+^ n ∘ z) (hx : |x| ≤ n) :
-    x.count 'b' = 0 := by
-  induction' x with s w ih generalizing n
-  · simp_all only [Word.length, Nat.zero_le, Word.count]
-  · specialize ih (n - 1)
-    simp_all only [Word.cat, Word.length, Word.count, ↓Char.isValue]
-    have ha : s = 'a' := by
-      clear ih
-      match n with
-      | 0 => simp_all only [cat, le_zero_eq, Nat.add_eq_zero, succ_ne_self, false_and]
-      | n + 1 =>
-        simp_all only [cat, add_eq, Nat.add_zero, cons.injEq]
-    simp_all only [↓Char.isValue, Char.reduceEq, ↓reduceIte]
-    subst ha
-    match n with
-    | 0 =>
-      subst hz
-      simp_all only [le_zero_eq, Nat.add_eq_zero, succ_ne_self, false_and]
-    | n + 1 =>
-      simp only [Nat.add_one_sub_one, ↓Char.isValue] at ih
-      rw [Symbol.pow] at hz
-      simp_all only [not_false_eq_true, cat, cons.injEq, true_and, forall_true_left, ↓Char.isValue]
-      exact ih (by omega)
-
-lemma not_pump : ¬pumping_property anbn_lang := by
-  rw [pumping_property]
-  push_neg  -- push_neg first
-  intro n hpos -- introduce n, and the hypothesis that n > 0
-
-  let z : Word := ('a' ^+^ n) ∘ ('b' ^+^ n) -- we need to use a fitting word
-  -- we'll need to show that the word is actually an element of anbn
-  have hzinanbn : z ∈ anbn := by
-    rw [anbn, Set.mem_setOf_eq]
-    use n
-  use z
-  -- simp only [gt_iff_lt, ge_iff_le]
-  -- we now need to show every conjunct
-  constructor
-  · exact hzinanbn
-  · -- we only need this 'have' because we don't have access to 'set' rather than let
-    have heq : z = 'a' ^+^ n ∘ 'b' ^+^ n := rfl
-    -- now we need to handle this inner conjunction
-    constructor
-    · -- showing that the length of z is actually greater than n - fairly trivial step
-      rw [heq, Word.cat_len, Symbol.pow_len, Symbol.pow_len]
-      omega
-    · -- main part of the proof!
-      intro u v w hcons hlenlower hv
-      use 2
-      -- it's obvious that v doesn't contain any b's, but we have to show it!
-      have honlyas : v.count 'b' = 0 := by
-        clear hv
-        -- this simp_all simplifies the proof state for us
-        simp_all only [gt_iff_lt, z, ↓Char.isValue]
-        have huv : (u ∘ v).count 'b' = 0 := by
-          symm at hcons
-          rw [← Word.cat_assoc] at hcons
-          -- might need to proof the cons_a lemma in the lemma section!
-          apply Word.cons_a n (u ∘ v) w ('b' ^+^ n) hcons hlenlower
-        exact (@Word.cat_count_zero 'b' u v huv).right
-      -- this is almost as obvious, but much more involved to show!
-      have hatleastonea : v.count 'a' > 0 := by
-        have hzcharsinab := anbn_lang.word_constraint z hzinanbn
-        -- simp to remove the .Alphabet thing
-        simp only [anbn_lang, ↓Char.isValue] at hzcharsinab
-        -- since v is a subword of z, its characters will be a subset of z's
-        have hsub : v.chars ⊆ z.chars := by
-          have hleft := Word.cat_char_subset_left v w
-          have hright := Word.cat_char_subset_right u (v ∘ w)
-          rw [hcons]
-          intro c hc
-          exact hright (hleft hc)
-        -- since z's characters are 'a' and 'b'
-        have hvchars : v.chars ⊆ {'a', 'b'} := subset_trans hsub hzcharsinab
-        -- clearing a bunch of hypotheses that will only be a distraction otherwise
-        clear hzinanbn hlenlower hcons heq u w z hpos n hzcharsinab hsub
-        -- from here on out we need a fairly lengthy induction
-        induction' v with s w ih
-        · simp_all only [Word.length, Nat.le_zero_eq, Nat.succ_ne_self]
-        · simp_all only [gt_iff_lt, Word.length, Nat.le_add_right, Word.count, ↓Char.isValue]
-          generalize w.count 'a' = n at *
-          split_ifs with hs
-          · exact Nat.le_add_right 1 n
-          · have hsb : s = 'b' := by
-              -- once again clearing unnecessary hypotheses
-              clear ih honlyas n
-              rw [Word.chars] at hvchars
-              have hsab := (Set.union_subset_iff.mp hvchars).left
-              -- with the preparatory work done, simp_all can take care of the rest
-              simp_all only [Set.singleton_union, Set.singleton_subset_iff, Set.mem_insert_iff,
-                Set.mem_singleton_iff, false_or]
-            split_ifs at honlyas with h
-            · simp_all only [Nat.add_eq_zero_iff, Nat.succ_ne_self, false_and]
-            · simp_all only
-      -- now we can proceed with the rest of the proof
-      -- mind that our main hypotheses right now are honlyas and hatleastonea,
-      -- and those reflect the steps in the proof that we worked through first
-      intro hin
-      -- we can do the next rewrite with a separate lemma!
-      simp only [Word.pow, Word.cat_eps, Set.mem_setOf_eq, anbn_lang] at hin
-      -- another big rewrite
-      simp_all only [gt_iff_lt, Word.cat_assoc, z, ↓Char.isValue]
-      -- clearing a few unneeded hypotheses
-      clear hlenlower hzinanbn hv hpos z
-      rcases hin with ⟨m, hm⟩
-      have heven : (u ∘ v ∘ v ∘ w).count 'a' = (u ∘ v ∘ v ∘ w).count 'b' := by
-        clear hatleastonea honlyas hcons
-        simp_all only [Word.cat_count, Symbol.pow_count, ite_true, ite_false, Nat.add_zero, Nat.zero_add, Char.reduceEq]
-      have huneven : (u ∘ v ∘ v ∘ w).count 'a' ≠ (u ∘ v ∘ v ∘ w).count 'b' := by
-        simp only [Word.cat_count, ne_eq, ↓Char.isValue]
-        intro heq
-        have hcount : (u ∘ v ∘ w).count 'a' = (u ∘ v ∘ w).count 'b' := by
-          rw [← hcons]
-          clear hcons
-          simp_all only [Nat.zero_add, Word.cat_count, Symbol.pow_count, ite_true, ite_false,
-            Nat.add_zero, Nat.add_zero, Nat.zero_add, Char.reduceEq]
-        simp only [Word.cat_count, ↓Char.isValue] at hcount
-        have hgoal : v.count 'a' = v.count 'b' := by
-          omega
-        simp_all only [lt_self_iff_false]
-      exact huneven heven
