Game/FormalLanguages/Lemmas.lean
@@ -1,0 +1,192 @@
+import Game.FormalLanguages.BasicDefinitions
+
+open Nat
+namespace Regular
+@[simp]
+lemma Word.cat_eps (w : Word) : w ∘ .ε = w := by
+  induction' w with s w ih
+  · rw [cat]
+  · rw [cat, ih]
+
+@[simp]
+lemma Word.cat_assoc (x y z : Word) : (x ∘ y) ∘ z = x ∘ y ∘ z := by
+  induction' x with s w ih <;> simp_all only [cat]
+
+@[simp]
+lemma Word.cat_count {s : Char} (x y : Word) :
+    (x ∘ y).count s = x.count s + y.count s := by
+  induction' x with s' w ih
+  · simp_all only [cat, count, Nat.zero_add]
+  · rw [count]
+    simp_all only [cat, count]
+    split
+    next h =>
+      omega
+    next h => simp_all only
+
+@[simp]
+lemma Word.cat_count_zero {s : Char} (x y : Word) :
+    (x ∘ y).count s = 0 → x.count s = 0 ∧ y.count s = 0 := by
+  intro hcatcount
+  apply And.intro <;> simp_all only [cat_count, Nat.add_eq_zero_iff]
+
+lemma Word.cat_char_subset_left (x y : Word) :
+    x.chars ⊆ (x ∘ y).chars := by
+  simp only [cat_chars, Set.subset_union_left]
+
+lemma Word.cat_char_subset_right (x y : Word) :
+    y.chars ⊆ (x ∘ y).chars := by
+  simp only [cat_chars, Set.subset_union_right]
+
+lemma Word.cat_len (x y : Word) :
+    |(x ∘ y)| = |x| + |y| := by
+  induction' x with s x ih
+  · simp only [cat, length, Nat.zero_add]
+  · rw [Word.length, Nat.add_assoc, ← ih]
+    simp_all only [length]
+
+
+@[simp]
+lemma Symbol.pow_len {s : Char} (n : ℕ) : |s ^ n| = n := by
+  induction' n with n ih
+  · rfl
+  · simp only [pow, Word.length]
+    rw [ih]
+    exact Nat.one_add _
+
+@[simp]
+lemma Symbol.pow_count {s₁ s₂ : Char} (n : ℕ) :
+    (s₁ ^ n).count s₂ = if s₁ = s₂ then n else 0 := by
+  induction' n with n ih
+  · simp_all only [pow, Word.count, ite_self]
+  · simp_all only [pow, Word.count, ↓reduceIte]
+    split
+    next h =>
+      subst h
+      simp_all only [↓reduceIte]
+      omega
+    next h => simp_all only [↓reduceIte]
+
+
+--set_option tactic.simp.trace true
+lemma Word.cons_a (n : ℕ) (x y z : Word) (hz : x ∘ y = ('a' ^ n) ∘ z) (hx : |x| ≤ n) :
+    x.count 'b' = 0 := by
+  induction' x with s w ih generalizing n
+  · simp_all only [Word.length, Nat.zero_le, Word.count]
+  · specialize ih (n - 1)
+    simp_all [Word.cat, Word.length, Word.count, Char.isValue]
+    have ha : s = 'a' := by
+      clear ih
+      match n with
+      | 0 => simp_all only [cat, le_zero_eq, Nat.add_eq_zero, succ_ne_self, false_and]
+      | n + 1 =>
+        simp_all only [cat, add_eq, Nat.add_zero, cons.injEq]
+    simp_all only [↓Char.isValue, Char.reduceEq, ↓reduceIte]
+    subst ha
+    match n with
+    | 0 =>
+      subst hz
+      simp_all only [le_zero_eq, Nat.add_eq_zero, succ_ne_self, false_and]
+    | n + 1 =>
+      simp only [Nat.add_one_sub_one, Char.isValue] at ih
+      rw [Symbol.pow] at hz
+      simp_all only [not_false_eq_true, cat, cons.injEq, true_and, forall_true_left, Char.isValue]
+      exact ih (by omega)
+
+lemma not_pump : ¬pumping_property anbn_lang := by
+  rw [pumping_property]
+  push_neg  -- push_neg first
+  intro n hpos -- introduce n, and the hypothesis that n > 0
+
+  let z : Word := ('a' ^ n) ∘ ('b' ^ n) -- we need to use a fitting word
+  -- we'll need to show that the word is actually an element of anbn
+  have hzinanbn : z ∈ anbn := by
+    rw [anbn, Set.mem_setOf_eq]
+    use n
+  use z
+  -- simp only [gt_iff_lt, ge_iff_le]
+  -- we now need to show every conjunct
+  constructor
+  · exact hzinanbn
+  · -- we only need this 'have' because we don't have access to 'set' rather than let
+    have heq : z = ('a' ^ n) ∘ 'b' ^ n := rfl
+    -- now we need to handle this inner conjunction
+    constructor
+    · -- showing that the length of z is actually greater than n - fairly trivial step
+      rw [heq, Word.cat_len, Symbol.pow_len, Symbol.pow_len]
+      omega
+    · -- main part of the proof!
+      intro u v w hcons hlenlower hv
+      use 2
+      -- it's obvious that v doesn't contain any b's, but we have to show it!
+      have honlyas : v.count 'b' = 0 := by
+        clear hv
+        -- this simp_all simplifies the proof state for us
+        simp_all only [gt_iff_lt, z, ↓Char.isValue]
+        have huv : (u ∘ v).count 'b' = 0 := by
+          symm at hcons
+          rw [← Word.cat_assoc] at hcons
+          -- might need to proof the cons_a lemma in the lemma section!
+          apply Word.cons_a n (u ∘ v) w ('b' ^ n) hcons hlenlower
+        exact (@Word.cat_count_zero 'b' u v huv).right
+      -- this is almost as obvious, but much more involved to show!
+      have hatleastonea : v.count 'a' > 0 := by
+        have hzcharsinab := anbn_lang.word_constraint z hzinanbn
+        -- simp to remove the .Alphabet thing
+        simp only [anbn_lang, ↓Char.isValue] at hzcharsinab
+        -- since v is a subword of z, its characters will be a subset of z's
+        have hsub : v.chars ⊆ z.chars := by
+          have hleft := Word.cat_char_subset_left v w
+          have hright := Word.cat_char_subset_right u (v ∘ w)
+          rw [hcons]
+          intro c hc
+          exact hright (hleft hc)
+        -- since z's characters are 'a' and 'b'
+        have hvchars : v.chars ⊆ {'a', 'b'} := subset_trans hsub hzcharsinab
+        -- clearing a bunch of hypotheses that will only be a distraction otherwise
+        clear hzinanbn hlenlower hcons heq u w z hpos n hzcharsinab hsub
+        -- from here on out we need a fairly lengthy induction
+        induction' v with s w ih
+        · simp_all only [Word.length, Nat.le_zero_eq, Nat.succ_ne_self]
+        · simp_all only [gt_iff_lt, Word.length, Nat.le_add_right, Word.count, ↓Char.isValue]
+          generalize w.count 'a' = n at *
+          split_ifs with hs
+          · exact Nat.le_add_right 1 n
+          · have hsb : s = 'b' := by
+              -- once again clearing unnecessary hypotheses
+              clear ih honlyas n
+              rw [Word.chars] at hvchars
+              have hsab := (Set.union_subset_iff.mp hvchars).left
+              -- with the preparatory work done, simp_all can take care of the rest
+              simp_all only [Set.singleton_union, Set.singleton_subset_iff, Set.mem_insert_iff,
+                Set.mem_singleton_iff, false_or]
+            split_ifs at honlyas with h
+            · simp_all only [Nat.add_eq_zero_iff, Nat.succ_ne_self, false_and]
+            · simp_all only
+      -- now we can proceed with the rest of the proof
+      -- mind that our main hypotheses right now are honlyas and hatleastonea,
+      -- and those reflect the steps in the proof that we worked through first
+      intro hin
+      -- we can do the next rewrite with a separate lemma!
+      simp only [Word.pow, Word.cat_eps, Set.mem_setOf_eq, anbn_lang] at hin
+      -- another big rewrite
+      simp_all only [gt_iff_lt, Word.cat_assoc, z, ↓Char.isValue]
+      -- clearing a few unneeded hypotheses
+      clear hlenlower hzinanbn hv hpos z
+      rcases hin with ⟨m, hm⟩
+      have heven : (u ∘ v ∘ v ∘ w).count 'a' = (u ∘ v ∘ v ∘ w).count 'b' := by
+        clear hatleastonea honlyas hcons
+        simp_all only [Word.cat_count, Symbol.pow_count, ite_true, ite_false, Nat.add_zero, Nat.zero_add, Char.reduceEq]
+      have huneven : (u ∘ v ∘ v ∘ w).count 'a' ≠ (u ∘ v ∘ v ∘ w).count 'b' := by
+        simp only [Word.cat_count, ne_eq, ↓Char.isValue]
+        intro heq
+        have hcount : (u ∘ v ∘ w).count 'a' = (u ∘ v ∘ w).count 'b' := by
+          rw [← hcons]
+          clear hcons
+          simp_all only [Nat.zero_add, Word.cat_count, Symbol.pow_count, ite_true, ite_false,
+            Nat.add_zero, Nat.add_zero, Nat.zero_add, Char.reduceEq]
+        simp only [Word.cat_count, ↓Char.isValue] at hcount
+        have hgoal : v.count 'a' = v.count 'b' := by
+          omega
+        simp_all only [lt_self_iff_false]
+      exact huneven heven
