Game/Levels/Lemmas/L02_cat_eps.lean
@@ -14,20 +14,20 @@ TheoremTab "cat"
 TheoremDoc Regular.cat_eps as "cat_eps" in "cat"
 
 /-- Concatenation of words: for two words w₁ and w₂, the concatenation w₁ and w₂ yields w₁w₂. -/
-DefinitionDoc Regular.Word.cat as "cat"
+DefinitionDoc Regular.Word.cat as "Word.cat"
 
 /-- A word over an alphabet, i.e. a string of symbols from that alphabet. -/
 DefinitionDoc Word as "Word"
 
 NewDefinition Word Regular.Word.cat
 
---TheoremDoc Regular.Word.cat as "Word.cat" in "Word"
-
---NewTheorem Regular.Word.cat
-
 Statement cat_eps (w : Word) : w.cat .ε = w := by
+  Hint "This proof calls for an induction! Try starting with `induction' w with s w ih`."
   induction' w with s w ih
-  · rw [Word.cat]
-  · rw [Word.cat, ih]
+  · Hint "This is essentially true by definition of `Word.cat`."
+    Hint (hidden := true) "`rw [Word.cat]`."
+    rw [Word.cat]
+  · Hint (hidden := true) "`rw [Word.cat, ih]`."
+    rw [Word.cat, ih]
 
 Conclusion "Good!"
