Game/Levels/Lemmas/L03_cat_assoc.lean
@@ -15,6 +15,12 @@ TheoremDoc Regular.cat_assoc as "cat_assoc" in "cat"
 
 
 Statement cat_assoc (x y z : Word) : (x ∘ y) ∘ z = x ∘ y ∘ z := by
-  induction' x with s w ih <;> simp_all only [Word.cat]
+  Hint (hidden := true) "Once again, start with `inductino' {x} with s w ih`."
+  induction' x with s w ih
+  · Hint (hidden := true) "Either rewrite with `Word.cat` multiple times, or just
+    use `simp [Word.cat]`."
+    simp [Word.cat]
+  · Hint (hidden := true) "Rewriting with `Word.cat` and then with `ih` works, or just use `simp_all [Word.cat]`."
+    simp_all [Word.cat]
 
 Conclusion "Good! Incidentally, we've just shown that strings together with concatenation form a monoid."
