Game/Levels/Lemmas/L04_gap.lean
@@ -10,6 +10,12 @@ Introduction "Let's prove a simple lemma: concatenating any word with the empty 
 
 namespace Regular
 
+Statement cat_chars (x y : Word) : (x ∘ y).chars = x.chars ∪ y.chars := by
+  induction' x with s w ih
+  · simp only [Word.cat, Word.chars, Set.empty_union]
+  · rw [Word.chars, Word.cat, Word.chars, ih]
+    rw [Set.union_assoc]
+
 Statement (x y z : Word) : (x ∘ y) ∘ z = x ∘ y ∘ z := by
   induction' x with s w ih <;> simp_all only [Word.cat]
 
