Game/Levels/Lemmas/L05_cat_count.lean
@@ -15,18 +15,25 @@ is the same as counting the occurrences in both subwords and adding them up.
 TheoremDoc Regular.cat_count as "cat_count" in "cat"
 
 /-- Counts how often a character occurs in a word. -/
-DefinitionDoc Regular.Word.count as "count"
+DefinitionDoc Regular.Word.count as "Word.count"
 
 NewDefinition Regular.Word.count
 
 Statement cat_count {s : Char} (x y : Word) :
     (x ∘ y).count s = x.count s + y.count s := by
+  Hint (hidden := true) "Start with `induction' x with s' w ih`."
   induction' x with s' w ih
-  · simp_all only [Word.cat, Word.count, Nat.zero_add]
-  · rw [Word.count]
-    simp_all only [Word.cat, Word.count]
+  · Hint (hidden := true) "Utilize `Word.cat` and `Word.count`."
+    Hint (hidden := true) "`simp [Word.cat, Word.count]`"
+    simp [Word.cat, Word.count]
+  · Hint "Remember you can use the tactic `split_ifs` to handle if statements."
+    Hint (hidden := true) "`simp [Word.cat, Word.count]`"
+    simp [Word.cat, Word.count]
+    Hint (hidden := true) "`split_ifs with h`"
     split_ifs with h
-    · omega
-    · simp_all only
+    · Hint (hidden := true) "`omega` will solve this goal directly!"
+      omega
+    · Hint (hidden := true) "`exact {ih}` closes the goal immediately."
+      exact ih
 
 Conclusion "Good!"
