Game/Levels/Lemmas/L06_cat_count_zero.lean
@@ -14,7 +14,15 @@ TheoremDoc Regular.cat_count_zero as "cat_count_zero" in "cat"
 
 Statement cat_count_zero {s : Char} (x y : Word) :
     (x ∘ y).count s = 0 → x.count s = 0 ∧ y.count s = 0 := by
+  Hint "Let's start out by introducing the antecedent: `intro hcatcount`"
   intro hcatcount
-  apply And.intro <;> simp_all only [cat_count, Nat.add_eq_zero_iff]
+  Hint "To split the conjunction, let's use the `constructor` tactic."
+  constructor
+  · Hint "Use the theorem `Nat.add_eq_zero`"
+    Hint (hidden := true) "simp_all [cat_count, Nat.add_eq_zero]"
+    simp_all [cat_count, Nat.add_eq_zero]
+  · Hint "Use the theorem `Nat.add_eq_zero_iff`"
+    Hint (hidden := true) "simp_all [cat_count, Nat.add_eq_zero_iff]"
+    simp_all [cat_count, Nat.add_eq_zero_iff]
 
 Conclusion "Good!"
