Game/Levels/NonregProofs/L02_Proof.lean
@@ -1,4 +1,4 @@
-import Game.Levels.Lemmas.L09_pow_count
+import Game.Levels.Lemmas.L10_cons_a
 import Game.Metadata
 
 World "NonregProofs"
@@ -29,8 +29,8 @@ Statement : ¬pumping_property anbn_lang := by
   Hint "We can now replicate the initial 'let n > 0' part of the proof with `intro n hpos`."
   intro n hpos
   Hint "The word we want to use is z = aⁿbⁿ.
-  Let's introduce it with `let z : Word := 'a' ^+^ {n} ∘ 'b' ^+^ {n}`"
-  let z : Word := 'a' ^+^ n ∘ 'b' ^+^ n
+  Let's introduce it with `set z : Word := ('a' ^ n) ∘ 'b' ^ n with hz`"
+  set z : Word := ('a' ^ n) ∘ 'b' ^ n with hz
   Hint "We will need to show that z is actually an element of the language anbn in
   a second, so let's introduce that as a new hypothesis: `have hzinanbn : z ∈ anbn`."
   have hzinanbn : z ∈ anbn
@@ -44,13 +44,6 @@ Statement : ¬pumping_property anbn_lang := by
   · Hint "`exact {hzinanbn}` closes the goal directly."
     exact hzinanbn
   · -- we only need this 'have' because we don't have access to 'set' rather than let
-    Hint "Since we're using an earlier Lean version for several reasons, we don't
-    have access to the `set` tactic, which would have given us a hypothesis that
-    `{z}` is indeed equal to aⁿbⁿ. However, we introduced `{z}` with the `let` tactic,
-    so we will need to prove that hypothesis separately:
-
-    `have heq : {z} = 'a' ^+^ n ∘ 'b' ^+^ n := rfl`"
-    have heq : z = 'a' ^+^ n ∘ 'b' ^+^ n := rfl
     Hint "We once again use `constructor` to handle the conjunction."
     constructor
     · -- showing that the length of z is actually greater than n - fairly trivial step
@@ -59,8 +52,8 @@ Statement : ¬pumping_property anbn_lang := by
       and then use the `omega` tactic once you arrive at a proof state of the form
       `n + n > n`."
       Hint (hidden := true) "The exact hypotheses for rewriting that you should use
-      are `{heq}`, `Word.cat_len`, `Symbol.pow_len`, and `Symbol.pow_len` again."
-      rw [heq, Word.cat_len, Symbol.pow_len, Symbol.pow_len]
+      are `{hz}`, `cat_len`, `pow_len`, and `pow_len` again."
+      rw [hz, cat_len, pow_len, pow_len]
       omega
     ·
       Hint "We can finally get to the main part of the proof! First of all, we need
@@ -76,7 +69,7 @@ Statement : ¬pumping_property anbn_lang := by
       -- it's obvious that v doesn't contain any b's, but we have to show it!
       Hint "In our paper proof, we made an argument for why there are no b's in `{v}`. For our formalization, let's have this as a separate hypothesis:
 
-      `have honlyas: {v}.count 'b' = 0`"
+      `have honlyas : {v}.count 'b' = 0`"
       have honlyas : v.count 'b' = 0
       ·
         -- this simp_all simplifies the proof state for us
@@ -89,20 +82,20 @@ Statement : ¬pumping_property anbn_lang := by
         ·
           Hint "We need to utilize the associativity that we proved earlier:
 
-          `rw [← Word.cat_assoc]`
+          `rw [← Word.cat_assoc] at hcons`
 
           Following that, use the tactic `symm at {hcons}`"
-          rw [← Word.cat_assoc] at hcons
+          rw [← cat_assoc] at hcons
           symm at hcons
           -- might need to proof the cons_a lemma in the lemma section!
           Hint "For this specific situation, the lemma `Word.cons_a` is already provided to us, so you can finish the subproof with
 
-          `apply Word.cons_a {n} ({u} ∘ {v}) {w} ('b' ^+^ {n}) {hcons} {hlenlower}`"
-          apply Word.cons_a n (u ∘ v) w ('b' ^+^ n) hcons hlenlower
+          `apply Word.cons_a {n} ({u} ∘ {v}) {w} ('b' ^ {n}) {hcons} {hlenlower}`"
+          apply cons_a n (u ∘ v) w ('b' ^ n) hcons hlenlower
         Hint "We can now use the fresh hypothesis `{huv}`:
 
         `exact (@Word.cat_count_zero 'b' {u} {v} {huv}).right`"
-        exact (@Word.cat_count_zero 'b' u v huv).right
+        exact (@cat_count_zero 'b' u v huv).right
       -- this is almost as obvious, but much more involved to show!
       Hint "For the next step of our proof, we showed that `{v}` contained at least
       one 'a'. This will unfortunately be much more involved to show!"
@@ -113,22 +106,22 @@ Statement : ¬pumping_property anbn_lang := by
         simp only [anbn_lang, ↓Char.isValue] at hzcharsinab
         -- since v is a subword of z, its characters will be a subset of z's
         have hsub : v.chars ⊆ z.chars := by
-          have hleft := Word.cat_char_subset_left v w
-          have hright := Word.cat_char_subset_right u (v ∘ w)
+          have hleft := cat_char_subset_left v w
+          have hright := cat_char_subset_right u (v ∘ w)
           rw [hcons]
           intro c hc
           exact hright (hleft hc)
         -- since z's characters are 'a' and 'b'
         have hvchars : v.chars ⊆ {'a', 'b'} := subset_trans hsub hzcharsinab
         -- clearing a bunch of hypotheses that will only be a distraction otherwise
-        clear hzinanbn hlenlower hcons heq u w z hpos n hzcharsinab hsub
+        clear hzinanbn hlenlower hcons hz u w z hpos n hzcharsinab hsub
         -- from here on out we need a fairly lengthy induction
         induction' v with s w ih
         · simp_all only [Word.length, Nat.le_zero_eq, Nat.succ_ne_self]
         · simp_all only [gt_iff_lt, Word.length, Nat.le_add_right, Word.count, ↓Char.isValue]
           generalize w.count 'a' = n at *
           split_ifs with hs
-          · exact Nat.le_add_right 1 n
+          · omega
           · have hsb : s = 'b' := by
               -- once again clearing unnecessary hypotheses
               clear ih honlyas n
@@ -145,24 +138,24 @@ Statement : ¬pumping_property anbn_lang := by
       -- and those reflect the steps in the proof that we worked through first
       intro hin
       -- we can do the next rewrite with a separate lemma!
-      simp only [Word.pow, Word.cat_eps, Set.mem_setOf_eq, anbn_lang] at hin
+      simp only [Word.pow, cat_eps, Set.mem_setOf_eq, anbn_lang] at hin
       -- another big rewrite
-      simp_all only [gt_iff_lt, Word.cat_assoc, z, ↓Char.isValue]
+      simp_all only [gt_iff_lt, cat_assoc, z, ↓Char.isValue]
       -- clearing a few unneeded hypotheses
       clear hlenlower hzinanbn hv hpos z
       rcases hin with ⟨m, hm⟩
       have heven : (u ∘ v ∘ v ∘ w).count 'a' = (u ∘ v ∘ v ∘ w).count 'b' := by
         clear hatleastonea honlyas hcons
-        simp_all only [Word.cat_count, Symbol.pow_count, ite_true, ite_false, Nat.add_zero, Nat.zero_add, Char.reduceEq]
+        simp_all only [cat_count, pow_count, ite_true, ite_false, Nat.add_zero, Nat.zero_add, Char.reduceEq]
       have huneven : (u ∘ v ∘ v ∘ w).count 'a' ≠ (u ∘ v ∘ v ∘ w).count 'b' := by
-        simp only [Word.cat_count, ne_eq, ↓Char.isValue]
+        simp only [cat_count, ne_eq, ↓Char.isValue]
         intro heq
         have hcount : (u ∘ v ∘ w).count 'a' = (u ∘ v ∘ w).count 'b' := by
           rw [← hcons]
           clear hcons
-          simp_all only [Nat.zero_add, Word.cat_count, Symbol.pow_count, ite_true, ite_false,
+          simp_all only [Nat.zero_add, cat_count, pow_count, ite_true, ite_false,
             Nat.add_zero, Nat.add_zero, Nat.zero_add, Char.reduceEq]
-        simp only [Word.cat_count, ↓Char.isValue] at hcount
+        simp only [cat_count, ↓Char.isValue] at hcount
         have hgoal : v.count 'a' = v.count 'b' := by
           omega
         simp_all only [lt_self_iff_false]
